More work on basic format combinators.

src/Narcissus/Formats/Base/SequenceFormat.v
@@ -8,12 +8,12 @@ Require Import
 
 Section SequenceFormat.
 
-  Context {S : Type}. (* Source Type *)
   Context {T : Type}. (* Target Type *)
   Context {cache : Cache}. (* State Type *)
   Context {monoid : Monoid T}. (* Target type is a monoid. *)
 
   Definition sequence_Format
+             {S : Type}
              (format1 format2 : FormatM S T)
     := (fun s env =>
           `(t1, env') <- format1 s env ;
@@ -21,433 +21,115 @@ Section SequenceFormat.
            ret (mappend t1 t2, env''))%comp.
 
   Definition sequence_Decode
-             {S' : Type}
+             {S S' : Type}
              (decode1 : DecodeM (S' * T) T)
              (decode2 : S' -> DecodeM S T)
     : DecodeM S T
     := (fun t env =>
           match decode1 t env with
-          | Some (s', t', env') => decode2 s' t' env
+          | Some (s', t', env') => decode2 s' t' env'
           | None => None
           end).
 
   Definition sequence_Encode
+             {S : Type}
              (encode1 encode2 : EncodeM S T)
     := (fun s env =>
           `(t1, env') <- encode1 s env ;
           `(t2, env'') <- encode2 s env';
           Some (mappend t1 t2, env'')).
 
-  Notation "x ++ y" := (sequence_Format _ x y) : format_scope .
+  Notation "x ++ y" := (sequence_Format x y) : format_scope .
 
-  Lemma sequeunce_Format_assoc
-        (format1 format2 format3 : FormatM S T)
-    : forall s env,
-      refineEquiv (sequence_Format (sequence_Format format1 format2) format3 s env)
-                  (sequence_Format format1 (sequence_Format format2 format3) s env).
+  Lemma CorrectEncoder_sequence
+        {S : Type}
+        (format1 format2 : FormatM S T)
+        (encode1 encode2 : EncodeM S T)
+        (encode1_correct : CorrectEncoder format1 encode1)
+        (encode1_consistent : (* If the first format produces *some*
+                                 environment that makes the second format
+                                 (and thus the composite format) non-empty,
+                                 the encoder must also produce an environment
+                                 that makes the second format non-empty. *)
+           forall s env tenv' tenv'',
+             format1 s env ∋ tenv'
+             -> format2 s (snd tenv') ∋ tenv''
+             -> exists tenv3 tenv4,
+                 encode1 s env = Some tenv3
+                 /\ format2 s (snd tenv3) ∋ tenv4)
+        (encode2_correct : CorrectEncoder format2 encode2)
+    : CorrectEncoder (format1 ++ format2)
+                     (sequence_Encode encode1 encode2).
   Proof.
-    unfold sequence_Format; intros.
-    rewrite refineEquiv_bind2_bind.
-    eapply refineEquiv_bind; [ reflexivity | ].
-    intro; rewrite refineEquiv_bind2_bind.
-    symmetry; rewrite refineEquiv_bind2_bind.
-    eapply refineEquiv_bind; [ reflexivity | ].
-    intro; rewrite refineEquiv_bind2_bind.
-    rewrite refineEquiv_bind2_unit.
-    eapply refineEquiv_bind; [ reflexivity | ].
-    intro; rewrite refineEquiv_bind2_unit; simpl.
-    rewrite mappend_assoc; reflexivity.
+    unfold CorrectEncoder, sequence_Encode, sequence_Format,
+    DecodeBindOpt, BindOpt in *; intuition; intros.
+    - destruct (encode1 a env) as [ [t1 xxenv] | ] eqn: ? ;
+        simpl in *; try discriminate.
+      destruct (encode2 a xxenv) as [ [t2 xxxenv] | ] eqn: ? ;
+        simpl in *; try discriminate; injections.
+      repeat computes_to_econstructor; eauto.
+    -  unfold Bind2 in *; computes_to_inv; destruct v;
+         destruct v0; simpl in *.
+       destruct (encode1 a env) as [ [t1 xxenv] | ] eqn: ? ;
+        simpl in *; try discriminate; eauto.
+       eapply H2; try eassumption.
+       destruct (encode2 a xxenv) as [ [t2' xxxenv] | ] eqn: ? ;
+        simpl in *; try discriminate; injections.
+       specialize (encode1_consistent _ _ _ _ H4 H4');
+         destruct_ex; split_and.
+       rewrite H6 in Heqo; injections; simpl in *.
+       destruct x0; elimtype False; eauto.
   Qed.
 
-  Lemma refineEquiv_under_sequence_Format
-        (format1 format2 format2' : FormatM S T)
-    : (forall s env, refineEquiv (format2 s env) (format2' s env))
-      -> forall s env,
-        refineEquiv (sequence_Format format1 format2 s env)
-                    (sequence_Format format1 format2' s env).
+  Lemma CorrectDecoder_sequence
+        {S S' : Type}
+        (f : S -> S')
+        (format1 : FormatM S' T)
+        (format2 : FormatM S T)
+        (decode1 : DecodeM (S' * T) T)
+        (decode2 : S' -> DecodeM S T)
+        (decode1_correct : CorrectDecoder_simpl ((Projection_Format (fun st => (fst st)) format1) ++ ?* ) decode1)
+        (decode2_correct : forall (s' : S'), CorrectDecoder_simpl format2 (decode2 s'))
+    : CorrectDecoder_simpl (Projection_Format f format1 ++ format2)
+                           (sequence_Decode decode1 decode2).
   Proof.
-    unfold sequence_Format; intros.
-    eapply refineEquiv_bind; [ reflexivity | ].
-    intro ab; destruct ab; simpl.
-    eapply refineEquiv_bind; [ apply H | reflexivity ].
-  Qed.
-
-  Lemma sequence_Format_format_correct_simpl'
-      (format1 format2 : FormatM A B)
-      (decode1 : DecodeM (A' * B) B)
-      (decode2 : A' -> DecodeM A B)
-      (decode1_pf : CorrectDecoder_simpl
-                      format1 ++
-                      (fun data_rest env binxenv =>
-                         exists bin', fst binxenv = mappend bin' (snd data_rest) /\
-                                      format1 (fst data_rest) env (bin', snd binxenv))
-                      decode1)
-      (decode2 : A' -> B -> CacheDecode -> option (A * CacheDecode))
-      (decode2_pf : forall proj,
-          CorrectDecoder_simpl (RestrictFormat format2 (fun data => project data = proj))
-                               (decode2 proj))
-  : CorrectDecoder_simpl
-      (fun (data : A) (env : CacheFormat) =>
-         sequence_Format _ (format1 (project data)) (format2 data) env
-      )%comp
-      (fun (bin : B) (env : CacheDecode) =>
-         `(proj, env') <- decode1 bin env;
-           decode2 (fst proj) (snd proj) env').
-Proof.
-  eapply CorrectDecoder_simpl_equiv_format; eauto.
-  eapply CorrectDecoder_simpl_equiv_decode; try eassumption.
-  eapply CorrectDecoder_simpl_no_inv.
-  eapply CorrectDecoder_simpl_strict_equiv.
-Abort.
-
-  Lemma CorrectDecoder_Enqueue
-    : CorrectDecoder_simpl (Enqueue_Format (decode).
-  Proof.
-    unfold CorrectDecoder_simpl, FMap_Decode, FMap_Format in *; split; intros.
-    { repeat (apply_in_hyp @unfold_computes; destruct_ex; intuition).
-      pose proof (g_inverts_f  _ _ _ _ H3 H4).
-      rewrite <- unfold_computes in H3.
-      eapply H1 in H3; destruct_ex; intuition eauto.
-      eexists; rewrite H5; simpl; intuition eauto.
-      subst; eauto.
-    }
-    { apply_in_hyp DecodeBindOpt_inv; destruct_ex; intuition.
-      eapply H2 in H3; eauto; injections.
-      destruct_ex; eexists; intuition eauto.
-      apply unfold_computes.
+    unfold CorrectDecoder_simpl, Projection_Format,
+    sequence_Decode, sequence_Format, FMap_Format; split; intros.
+    - unfold Bind2 in H0; computes_to_inv; subst.
+      repeat apply_in_hyp @unfold_computes.
+      destruct v; destruct v0; simpl in *.
+      destruct_ex; intuition; injections.
+      destruct decode1_correct as [? _].
+      destruct (decode2_correct (f data)) as [? _].
+      destruct (H0 env env' c (f data, t0) (mappend t t0)) as (xenv', (decode1_eq, Equiv_xenv));
+        eauto.
+      { unfold Projection_Format, FMap_Format, LaxTerminal_Format; repeat computes_to_econstructor; eauto.
+        apply unfold_computes; eexists; intuition eauto.
+        computes_to_econstructor. }
+      rewrite decode1_eq; eauto.
+    - destruct (decode1 bin env') as [ [ [s' t'] xenv'']  | ] eqn: ?; try discriminate.
+      destruct decode1_correct as [decode1_correct' decode1_correct].
+      specialize (decode2_correct s'); destruct decode2_correct as [_ decode2_correct].
+      generalize Heqo; intro Heqo'.
+      eapply decode1_correct in Heqo; eauto.
+      destruct_ex; split_and.
+      eapply decode2_correct in H0; eauto.
+      destruct_ex; split_and.
       eexists; intuition eauto.
-    }
-  Qed.
+      unfold Projection_Format, FMap_Format, LaxTerminal_Format, sequence_Format,
+        Bind2 in *; computes_to_inv.
+      repeat apply_in_hyp @unfold_computes.
+      destruct_ex; split_and; simpl in *.
+      injections; simpl in *.
+      computes_to_econstructor.
+      apply unfold_computes.
+      eexists; split; try reflexivity.
+      Focus 2.
+      computes_to_econstructor; eauto.
+      apply unfold_computes; eauto.
+      eauto.
+  Admitted.
 
-Lemma sequence_Format_format_correct
-      {A A' B}
-      {cache : Cache}
-      {P  : CacheDecode -> Prop}
-      {P_inv1 P_inv2 : (CacheDecode -> Prop) -> Prop}
-      (P_inv_pf : cache_inv_Property P (fun P => P_inv1 P /\ P_inv2 P))
-      (monoid : Monoid B)
-      (project : A -> A')
-      (predicate : A -> Prop)
-      (predicate' : A' -> Prop)
-      (predicate_rest' : A -> B -> Prop)
-      (predicate_rest : A' -> B -> Prop)
-      (format1 : A' -> CacheFormat -> Comp (B * CacheFormat))
-      (format2 : A -> CacheFormat -> Comp (B * CacheFormat))
-      (decode1 : B -> CacheDecode -> option (A' * B * CacheDecode))
-      (decode1_pf :
-         cache_inv_Property P P_inv1
-         -> CorrectDecoder
-              monoid predicate'
-              predicate_rest
-              format1 decode1 P)
-      (pred_pf : forall data, predicate data -> predicate' (project data))
-      (predicate_rest_impl :
-         forall a' b
-                a ce ce' ce'' b' b'',
-           computes_to (format1 a' ce) (b', ce')
-           -> project a = a'
-           -> predicate a
-           -> computes_to (format2 a ce') (b'', ce'')
-           -> predicate_rest' a b
-           -> predicate_rest a' (mappend b'' b))
-      (decode2 : A' -> B -> CacheDecode -> option (A * B * CacheDecode))
-      (decode2_pf : forall proj,
-          predicate' proj ->
-          cache_inv_Property P P_inv2 ->
-          CorrectDecoder monoid
-                                  (fun data => predicate data /\ project data = proj)
-                                  predicate_rest'
-                                  format2
-                                  (decode2 proj) P)
-  : CorrectDecoder
-      monoid
-      (fun a => predicate a)
-      predicate_rest'
-      (fun (data : A) (env : CacheFormat) =>
-         sequence_Format _ (format1 (project data)) (format2 data)  env
-      )%comp
-      (fun (bin : B) (env : CacheDecode) =>
-         `(proj, rest, env') <- decode1 bin env;
-           decode2 proj rest env') P.
-Proof.
-  unfold cache_inv_Property in *; split.
-  { intros env env' xenv data bin ext ? env_pm pred_pm pred_pm_rest com_pf.
-    unfold sequence_Format, Bind2 in com_pf; computes_to_inv; destruct v;
-      destruct v0.
-    destruct (fun H' => proj1 (decode1_pf (proj1 P_inv_pf)) _ _ _ _ _ (mappend b0 ext) env_OK env_pm (pred_pf _ pred_pm) H' com_pf); intuition; simpl in *; injections; eauto.
-    setoid_rewrite <- mappend_assoc; rewrite H2.
-    simpl.
-    destruct (fun H'' => proj1 (decode2_pf (project data) (pred_pf _ pred_pm) H1)
-                               _ _ _ _ _ ext H4 H (conj pred_pm (eq_refl _)) H'' com_pf');
-      intuition; simpl in *; injections.
-    eauto. }
-  { intros.
-    destruct (decode1 bin env') as [ [ [? ?] ? ] | ] eqn : ? ;
-      simpl in *; try discriminate.
-    eapply (proj2 (decode1_pf (proj1 P_inv_pf))) in Heqo; eauto.
-    destruct Heqo as [? [? [? [? [? [? ?] ] ] ] ] ].
-    eapply (proj2 (decode2_pf a H5 (proj2 P_inv_pf))) in H2; eauto.
-    destruct H2 as [? ?]; destruct_ex; intuition; subst.
-    eexists; eexists; repeat split.
-    repeat computes_to_econstructor; eauto.
-    simpl; rewrite mappend_assoc; reflexivity.
-    eassumption.
-    eassumption.
-  }
-Qed.
+            End SequenceFormat.
 
-Lemma sequence_Format_format_correct_simpl
-      {A A' B}
-      {cache : Cache}
-      {monoid : Monoid B}
-      (project : A -> A')
-      (format1 : FormatM A' B)
-      (format2 : FormatM A B)
-      (decode1 : DecodeM (A' * B) B)
-      (*oblivious_decoder : forall bs data env bs' env',
-          decode1 bs env = Some (data, bs', env') ->
-          forall bs'', decode1 (mappend bs bs'') env = Some (data, mappend bs' bs'', env')*)
-      (decode1_pf : CorrectDecoder_simpl
-                      (fun data_rest env binxenv =>
-                         exists bin', fst binxenv = mappend bin' (snd data_rest) /\
-                                      format1 (fst data_rest) env (bin', snd binxenv))
-                      decode1)
-      (decode2 : A' -> B -> CacheDecode -> option (A * CacheDecode))
-      (decode2_pf : forall proj,
-          CorrectDecoder_simpl (RestrictFormat format2 (fun data => project data = proj))
-                               (decode2 proj))
-  : CorrectDecoder_simpl
-      (fun (data : A) (env : CacheFormat) =>
-         sequence_Format _ (format1 (project data)) (format2 data) env
-      )%comp
-      (fun (bin : B) (env : CacheDecode) =>
-         `(proj, env') <- decode1 bin env;
-           decode2 (fst proj) (snd proj) env').
-Proof.
-  split.
-  { intros; unfold sequence_Format, Bind2 in *; computes_to_inv;
-      destruct v; destruct v0; simpl in *; injections.
-    destruct decode1_pf.
-    destruct (H1 _ _ c (project data, b0) (mappend b b0) H) as [? [? ?] ].
-    apply unfold_computes.
-    rewrite unfold_computes in H0; simpl; eauto.
-    specialize (decode2_pf (project data)); destruct decode2_pf.
-    destruct (H5 c x xenv data b0 H4) as [? [? ?] ].
-    unfold RestrictFormat; rewrite unfold_computes; intuition.
-    rewrite H3; simpl; rewrite H7; eauto. }
-  { intros.
-    destruct (decode1 bin env') as [ [ [? ?] ? ] | ] eqn : ? ;
-      simpl in *; try discriminate.
-    eapply (proj2 decode1_pf) in Heqo; eauto.
-    destruct Heqo as [? [? ?] ].
-    apply unfold_computes in H1; intuition; simpl in *;
-      destruct_ex; intuition; subst.
-    eapply (proj2 (decode2_pf _)) in H0; eauto.
-    destruct H0 as [? ?]; destruct_ex; intuition; subst.
-    unfold RestrictFormat in H1; apply unfold_computes in H1; intuition.
-    rewrite H5.
-    unfold sequence_Format; eexists; intuition eauto.
-    repeat first [computes_to_econstructor
-                  | apply unfold_computes; eauto ]. }
-Qed.
-
-Lemma sequence_Format_format_correct_simpl'
-      {A A' B}
-      {cache : Cache}
-      {monoid : Monoid B}
-      (project : A -> A')
-      (format1 : FormatM A' B)
-      (format2 : FormatM A B)
-      (decode1 : DecodeM (A' * B) B)
-      (*oblivious_decoder : forall bs data env bs' env',
-          decode1 bs env = Some (data, bs', env') ->
-          forall bs'', decode1 (mappend bs bs'') env = Some (data, mappend bs' bs'', env')*)
-      (decode1_pf : CorrectDecoder_simpl
-                      (fun data_rest env binxenv =>
-                         exists bin', fst binxenv = mappend bin' (snd data_rest) /\
-                                      format1 (fst data_rest) env (bin', snd binxenv))
-                      decode1)
-      (decode2 : A' -> B -> CacheDecode -> option (A * CacheDecode))
-      (decode2_pf : forall proj,
-          CorrectDecoder_simpl (RestrictFormat format2 (fun data => project data = proj))
-                               (decode2 proj))
-  : CorrectDecoder_simpl
-      (fun (data : A) (env : CacheFormat) =>
-         sequence_Format _ (format1 (project data)) (format2 data) env
-      )%comp
-      (fun (bin : B) (env : CacheDecode) =>
-         `(proj, env') <- decode1 bin env;
-           decode2 (fst proj) (snd proj) env').
-Proof.
-  eapply CorrectDecoder_simpl_equiv_format; eauto.
-  eapply CorrectDecoder_simpl_equiv_decode; try eassumption.
-  eapply CorrectDecoder_simpl_no_inv.
-  eapply CorrectDecoder_simpl_strict_equiv.
-Abort.
-
-(* For decoding fixed fields that do no depend on the object *)
-(* being formatd, e.g. version numbers in an IP packet. This *)
-(* allows us to avoid polluting the data invariant with  *)
-(* extraneous clauses. *)
-
-(* SUGGESTION: If we're using a deterministic formatr, we *)
-(* could compare the binary values of the field instead of *)
-(* decoding and comparing. *)
-
-Lemma sequence_Format_format_correct_no_dep
-      {A A' B}
-      (* Need decideable equality on the type of the fixed field. *)
-      (A'_eq_dec : Query_eq A')
-      {cache : Cache}
-      {P  : CacheDecode -> Prop}
-      {P_inv1 P_inv2 : (CacheDecode -> Prop) -> Prop}
-      (P_inv_pf : cache_inv_Property P (fun P => P_inv1 P /\ P_inv2 P))
-      (monoid : Monoid B)
-      (a' : A')
-      (predicate : A -> Prop)
-      (predicate' : A' -> Prop)
-      (predicate_rest' : A -> B -> Prop)
-      (predicate_rest : A' -> B -> Prop)
-      (format1 : A' -> CacheFormat -> Comp (B * CacheFormat))
-      (format2 : A -> CacheFormat -> Comp (B * CacheFormat))
-      (decode1 : B -> CacheDecode -> option (A' * B * CacheDecode))
-      (decode1_pf :
-         cache_inv_Property P P_inv1
-         -> CorrectDecoder monoid predicate' predicate_rest
-                                    format1 decode1 P)
-      (predicate_a' : predicate' a')
-      (predicate_rest_impl :
-         forall a' b
-                a ce ce' ce'' b' b'',
-           computes_to (format1 a' ce) (b', ce')
-           -> predicate a
-           -> computes_to (format2 a ce') (b'', ce'')
-           -> predicate_rest' a b
-           -> predicate_rest a' (mappend b'' b))
-      (decode2 : B -> CacheDecode -> option (A * B * CacheDecode))
-      (decode2_pf :
-         predicate' a' ->
-         cache_inv_Property P P_inv2 ->
-         CorrectDecoder monoid
-                                 (fun data => predicate data)
-                                 predicate_rest'
-                                 format2
-                                 decode2 P)
-  : CorrectDecoder
-      monoid
-      (fun a => predicate a)
-      predicate_rest'
-      (fun (data : A) (env : CacheFormat) =>
-         sequence_Format _ (format1 a') (format2 data)  env
-      )%comp
-      (fun (bin : B) (env : CacheDecode) =>
-         `(a, rest, env') <- decode1 bin env;
-           (if A_eq_dec a a' then decode2 rest env' else None)) P.
-Proof.
-  unfold cache_inv_Property in *; split.
-  { intros env env' xenv data bin ext ? env_pm pred_pm pred_pm_rest com_pf.
-    unfold sequence_Format, Bind2 in com_pf; computes_to_inv; destruct v;
-      destruct v0.
-    destruct (fun H => proj1 (decode1_pf (proj1 P_inv_pf)) _ _ _ _ _ (mappend b0 ext) env_OK env_pm predicate_a' H com_pf); intuition; simpl in *; injections.
-    eapply predicate_rest_impl; eauto.
-    setoid_rewrite <- mappend_assoc; rewrite H2.
-    simpl.
-    destruct (A_eq_dec a' a'); try congruence.
-    subst.
-    destruct (fun H => proj1 H6 (*decode2_pf _ (conj (eq_refl _) predicate_a') H1*)
-                             _ _ _ _ _ ext H4 H pred_pm pred_pm_rest com_pf');
-      intuition; simpl in *; injections.
-    eauto. }
-  { intros.
-    destruct (decode1 bin env') as [ [ [? ?] ? ] | ] eqn : ? ;
-      simpl in *; try discriminate;
-        destruct (A_eq_dec a a'); try discriminate;
-          eapply (proj2 (decode1_pf (proj1 P_inv_pf))) in Heqo; eauto;
-            destruct Heqo; destruct_ex; intuition; subst;
-              eapply (proj2 H11 (*decode2_pf a' (conj (eq_refl _) H7) H5)*)) in H1; eauto;
-                destruct H1; destruct_ex; intuition; subst.
-    eexists; eexists; repeat split.
-    repeat computes_to_econstructor; eauto.
-    simpl; rewrite mappend_assoc; reflexivity.
-    eassumption.
-    eassumption.
-  }
-Qed.
-
-Lemma CorrectDecoderinish {A B}
-  : forall (cache : Cache)
-           (monoid : Monoid B)
-           (predicate : A -> Prop)
-           (rest_predicate : A -> B -> Prop)
-           (decode_inv : CacheDecode -> Prop)
-           (a : A)
-           (b : bool),
-    (forall a', predicate a' -> a' = a)
-    -> decides b (predicate a)
-    -> CorrectDecoder
-         monoid
-         predicate
-         rest_predicate
-         (fun a' envE => ret (mempty, envE))
-         (fun b' envD => if b then Some (a, b', envD) else None)
-         decode_inv.
-Proof.
-  unfold CorrectDecoder; split; intros.
-  - eexists env'; pose proof (H _ H2); subst; find_if_inside;
-      simpl in *; intuition eauto; computes_to_inv; injections.
-    rewrite mempty_left; eauto.
-    eassumption.
-  - find_if_inside; injections; try discriminate;
-      simpl in *; intuition eauto.
-    eexists; eexists; intuition eauto.
-    rewrite mempty_left; reflexivity.
-Qed.
-
-Lemma decides_and :
-  forall b b' P Q,
-    decides b P
-    -> decides b' Q
-    -> decides (andb b b') (P /\ Q).
-Proof.
-  destruct b; destruct b'; simpl in *; intuition.
-Qed.
-
-Lemma decides_assumption :
-  forall (P : Prop),
-    P -> decides true P.
-Proof. simpl in *; intuition. Qed.
-
-Lemma decides_eq_refl {A} :
-  forall (a : A), decides true (a = a).
-Proof. simpl in *; intuition. Qed.
-
-Lemma decides_dec_eq {A} :
-  forall (A_eqb : A -> A -> bool)
-         (A_eqb_sound : forall a a', a = a' <-> A_eqb a a' = true)
-         (a a' : A), decides (A_eqb a a') (a = a').
-Proof.
-  simpl in *; intros; pose proof (A_eqb_sound a a');
-    destruct (A_eqb a a'); simpl; intuition.
-Qed.
-
-Lemma decides_dec_lt
-  : forall n n', decides (if (Compare_dec.lt_dec n n') then true else false) (lt n n').
-Proof.
-  intros; find_if_inside; simpl; eauto.
-Qed.
-
-Lemma refine_If_Then_Else_ThenC
-  : forall (E B : Type) (monoid : Monoid B) (format1 format2 format3 : E -> Comp (B * E)) (env : E) b,
-    refine (((If b Then format1 Else format2) ThenC format3) env)
-           (If b Then ((format1 ThenC format3) env) Else ((format2 ThenC format3) env)).
-Proof.
-  intros; destruct b; reflexivity.
-Qed.
-
-Lemma refineEquiv_If_Then_Else_ThenC
-  : forall (E B : Type) (monoid : Monoid B) (format1 format2 format3 : E -> Comp (B * E)) (env : E) b,
-    refineEquiv (((If b Then format1 Else format2) ThenC format3) env)
-                (If b Then ((format1 ThenC format3) env) Else ((format2 ThenC format3) env)).
-Proof.
-  intros; destruct b; reflexivity.
-Qed.
+            Notation "x ++ y" := (sequence_Format x y) : format_scope .
